@base <http://rightsstatements.org/vocab/> .
@prefix cc: <http://creativecommons.org/ns#> .
@prefix dc: <http://purl.org/dc/elements/1.1/> .
@prefix owl: <http://www.w3.org/2002/07/owl#> .
@prefix dcmitype: <http://purl.org/dc/dcmitype/> .
@prefix dcterms: <http://purl.org/dc/terms/> .
@prefix edm: <http://www.europeana.eu/schemas/edm/> .
@prefix foaf: <http://xmlns.com/foaf/0.1/> .
@prefix odrl: <http://www.w3c.org/community/odrl/two/vocab/2.1/> .
@prefix p3p: <http://www.w3.org/2002/01/p3prdfv1#> .
@prefix premiscopy: <http://id.loc.gov/vocabulary/preservation/copyrightStatus/> .
@prefix rdfs: <http://www.w3.org/2000/01/rdf-schema#> .
@prefix schema: <http://schema.org/> .
@prefix skos: <http://www.w3.org/2004/02/skos/core#> .
@prefix xsd: <http://www.w3.org/2001/XMLSchema#> .

# Metadata about the vocabulary itself

<0.0/> a skos:ConceptScheme ;
  dcterms:title "RightsStatements.org Standardized International Rights Statements"@en ;
  dcterms:title "RightsStatements.org Gestandaardiseerde Internationale Rechtenstatements"@nl ;
  dcterms:creator <irswg> ;
  dc:identifier "rscs" ;
  owl:versionInfo "0.0" ;
  dcterms:isReplacedBy <1.0/> ;
  skos:note "This is a fake version and should not be published or used in data."@en .

<irswg> a edm:Agent, foaf:Group ;
  foaf:name "International Rights Statements Working Group"@en ;
  skos:prefLabel "International Rights Statements Working Group"@en ;
  skos:prefLabel "Internationale Rechtenstatements Werkgroep"@nl ;
  foaf:homepage <http://rightsstatements.org/> .

# Information about the three "collections" of statements

<collection-ic/0.0/> a skos:Collection ;
  skos:prefLabel "rights statements for works that are in copyright"@en ;
  skos:prefLabel "rechtenstatements voor werken die auteursrechtelijk beperkt worden"@nl ;
  owl:versionInfo "0.0" ;
  skos:member <InC/0.0/> ;
  skos:member <InC-OW-EU/0.0/> ;
  skos:member <InC-RUU/0.0/> ;
  skos:member <InC-EDU/0.0/> ;
  skos:member <InC-NC/0.0/> .

<collection-pd/0.0/> a skos:Collection ;
  skos:prefLabel "rights statements for works that are not in copyright"@en ;
  skos:prefLabel "rechtenstatements voor werken die niet beperkt worden door het auteursrecht"@nl ;
  owl:versionInfo "0.0" ;
  skos:member <OOC-NC/0.0/> ;
  skos:member <NoC-CR/0.0/> ;
  skos:member <NoC-OKLR/0.0/> .

<collection-other/0.0/> a skos:Collection ;
  skos:prefLabel "other rights statements"@en ;
  skos:prefLabel "andere rechtenstatements"@nl ;
  owl:versionInfo "0.0" ;
  skos:member <NKC/0.0/> ;
  skos:member <CNE/0.0/> .

<InC/0.0/> a dcterms:RightsStatement, skos:Concept ;
  skos:prefLabel "In Copyright"@en ;
  skos:prefLabel "Auteursrechtelijk Beperkt"@nl ;
  dcterms:isReplacedBy <InC/1.0/> ;
  dcterms:modified "2016-02-25"^^xsd:date ;
  skos:closeMatch <http://www.europeana.eu/rights/rr-f/> ;
  skos:definition """This item is protected by copyright and/or related rights. 

You are free to use this item in any way that is permitted by the copyright and related rights legislation that applies to your use. 

For other uses you need to obtain permission from the rights-holder(s)."""@en ;
  skos:definition """Dit item is wordt door het auteursrecht of aanverwante rechten beperkt
Je bent vrij om dit item te gebruiken op manieren die worden toegestaan door de auteurswet of wetten op aanverwante rechten die op jou van toepassing zijn.

Voor andere gebruiken heb je toestemming van de rechthebbende nodig."""@nl ;

  skos:note "Unless expressly stated otherwise, the organization that has made this item available makes no warranties about the item and cannot guarantee the accuracy of this rights statement. You are responsible for your own use."@en ;
  skos:note "Tenzij expliciet aangegeven, de organisatie die dit artikel beschikbaar heeft gesteld geeft geen garanties over het item. Je bent verantwoordelijk voor je eigen gebruik."@nl ;
  skos:note "You may need to obtain other permissions for your intended use. For example, other rights such as publicity, privacy or moral rights may limit how you may use the material."@en ;
  skos:note "Het is mogelijk dat je meer toestemming moet verkrijgen voor je beoogde gebruik. Bijvoorbeeld, andere rechten als publiciteitsrechten, privacy recht, of morele rechten kunnen het mogelijke gebruik van dit item beperken."@nl ;
  skos:note "You may find additional information about the copyright status of the item on the website of the organization that has made the item available."@en ;
  skos:note "Je kan aanvullende informatie over de rechtenstatus van het item op de website van de organisatie vinden die het item beschikbaar heeft gesteld."@nl ;
  skos:scopeNote """This rights statement can be used for an item that is in copyright. Using this statement implies that the organization making this item available has determined that the item is in copyright and either: 
  * is the rights-holder, 
  * has obtained permission from the rightsholder(s) to make the work available or, 
  * makes the work available under an exception or limitation to copyright (including fair use) that entitles it to make the work available."""@en ;
  skos:scopeNote "Dit rechtenstatement kan gebruikt worden voor elk dat door het auteursrecht beperkt wordt. Het gebruik van dit statement impliceert dat de organisatie die dit item beschikbaar heeft gesteld bepaald heeft het item door het auteursrecht beperkt wordt. Ze zijn of de rechthebbende, hebben toestemming van de rechthebbende verkregen of mogen dit item beschikbaar stellen volgens de beperking en uitzonderingen van het auteursrecht dat op hun van toepassing is."@nl ;
  skos:relatedMatch premiscopy:cpr ;
  owl:versionInfo "0.0" ;
  dcterms:creator <irswg> ;
  dc:identifier "InC" ;
  skos:inScheme <0.0/> .

<InC-OW-EU/0.0/> a dcterms:RightsStatement, skos:Concept ;
  skos:prefLabel "In Copyright - EU Orphan Work"@en ;
  skos:prefLabel "Auteursrechtelijk Beperkt - EU Verweesd Werk"@nl ;
  dcterms:isReplacedBy <InC-OW-EU/1.0/> ;
  dcterms:modified "2016-02-25"^^xsd:date ;
  skos:closeMatch <http://www.europeana.eu/rights/orphan-work-eu/> ;
  skos:definition """This item has been identified as an orphan work in the country of first publication and in line with Directive 2012/28/EU of the European Parliament and of the Council of 25 October 2012 on certain permitted uses of orphan works.

For this item, either (a) no rights-holder(s) have been identified or (b) one or more rights-holder(s) have been identified but none have been located even though a diligent search for the rights-holder(s) has been conducted. The results of the diligent search are available in the EU Orphan Works Database. 

You are free to use this item in any way that is permitted by the copyright and related rights legislation that applies to your use."""@en ;
  skos:definition """Dit item is geïdentificeerd als een verweesd werk in het land van eerste publicatie en in lijn met de Europese richtlijn 2012/28/EU van het Europees Parlement en de Europese Raad van 25 oktober 2012 inzake bepaalde toegestane gebruikswijzen van verweesde werken.

Er is/zijn geen rechthebbende(n) van dit werk geïdentificeerd. Of als deze wel zijn geïdentificeerd dan zijn deze niet te localiseren ondanks een grondige zoektocht. Het resultaat van deze grondige zoektocht is te vinden in de EU verweesde werken database.

Je bent vrij om dit item te gebruiken op de manier die toegestaan zijn door he auteursrecht en aanverwante rechten volgende de wetten die op jou van toepassing zijn."""@nl ;
  skos:note "Unless expressly stated otherwise, the organization that has made this item available makes no warranties about the item and cannot guarantee the accuracy of this rights statement. You are responsible for your own use."@en ;
  skos:note "Tenzij expliciet aangegeven, de organisatie die dit artikel beschikbaar heeft gesteld geeft geen garanties over het item. Je bent verantwoordelijk voor je eigen gebruik."@nl ;
  skos:note "You may need to obtain other permissions for your intended use. For example, other rights such as publicity, privacy or moral rights may limit how you may use the material."@en ;
  skos:note "Het is mogelijk dat je meer toestemming moet verkrijgen voor je beoogde gebruik. Bijvoorbeeld, andere rechten als publiciteitsrechten, privacy recht, of morele rechten kunnen het mogelijke gebruik van dit item beperken."@nl ;
  skos:note "You may find additional information about the copyright status of the item on the website of the organization that has made the item available."@en ;
  skos:note "Je kan aanvullende informatie over de rechtenstatus van het item op de website van de organisatie vinden die het item beschikbaar heeft gesteld."@nl ;
  skos:note "If you have any information that can contribute to identifying or locating the rights-holder(s), please notify the organization that has made the item available."@en;
  skos:note "Neem contact op met de organisatie die dit item beschikbaar heeft gesteld als je enige informatie hebt over de auteursrechtelijk status van dit item dat kan bijdragen aan de identificering of localisering van de rechthebbende."@nl ;
  skos:scopeNote "This rights statement is intended for use with works that have been identified as Orphan Works in accordance with Directive 2012/28/EU of the European Parliament and of the Council of 25 October 2012 on certain permitted uses of orphan works. It can only be applied to works that are covered by the Directive: works published in the form of books, journals, newspapers, magazines or other writings as well as cinematographic or audiovisual works and phonograms (note: this excludes photography and visual arts). It can only be applied by data providers that are beneficiaries of the Directive: publicly accessible libraries, educational establishments and museums, archives, film or audio heritage institutions and public-service broadcasting organizations, established in one of the EU member states. The beneficiary is also expected to have registered the work in the EU Orphan Works Database maintained by OHIM."@en ;
  skos:scopeNote "Dit rechtenstatement is bedoeld voor het gebruik met werken die geïdentificeerd zijn als verweesde werken zoals bepaald in de Europese richtlijn 2012/28/EU van het Europees Parlement en de Europese Raad van 25 oktober 2012 inzake bepaalde toegestane gebruikswijzen van verweesde werken. De statement kan alleen toegepast worden op werken die bepaald zijn in de richtlijn: werken gepubliceerd als een boek, tijdschrift, krant, magazine, of andere geschreven werken. Maar ook cinematografische, audiovisuele werken en fonogrammen (dit sluit visuele kunst en fotografie uit). De statement kan alleen toegepast worden door data providers die begunstigd zijn in de richtlijn: Publiek toegankelijke bibliotheken, onderwijsinstellingen, musea, audiovisuele erfgoedinstellingen en publieke omroepen die gevestigd zijn in EU lidstaten. Van de begunstigden wordt verwacht dat ze het item in de OHIM EU Orphan Works Database hebben geregistreerd."@nl ;
  skos:relatedMatch premiscopy:cpr ;
  dcterms:creator <irswg> ;
  owl:versionInfo "0.0" ;
  dc:identifier "InC-OW-EU" ;
  skos:inScheme <0.0/> .

<InC-RUU/0.0/> a dcterms:RightsStatement, skos:Concept ;
  skos:prefLabel "In Copyright - Copyright Owner Unlocatable or Unidentifiable"@en ;
  skos:prefLabel "Auteursrechtelijk Beperkt – Rechthebbende is niet te identificeren of te vinden"@nl ;
  dcterms:isReplacedBy <InC-RUU/1.0/> ;
  dcterms:modified "2016-02-25"^^xsd:date ;
  skos:definition """This item is protected by copyright and/or related rights. However, for this item, either (a) no rights-holder(s) have been identified or (b) one or more rights-holder(s) have been identified but none have been located.

You are free to use this item in any way that is permitted by the copyright and related rights legislation that applies to your use."""@en ;
  skos:definition """"Het gebruik van dit item is beperkt door auteursrechten of naburige rechten. Alleen zijn er geen rechtehebbende(n) geïdentificeerd, deze kunnen niet gevonden worden.
  
Je bent vrij om dit item te gebruiken op de manier die toegestaan zijn door he auteursrecht en aanverwante rechten volgende de wetten die op jou van toepassing zijn."""@nl ;
  skos:note "Unless expressly stated otherwise, the organization that has made this item available makes no warranties about the item and cannot guarantee the accuracy of this rights statement. You are responsible for your own use."@en ;
  skos:note "Tenzij expliciet aangegeven, de organisatie die dit artikel beschikbaar heeft gesteld geeft geen garanties over het item. Je bent verantwoordelijk voor je eigen gebruik."@nl ;
  skos:note "You may need to obtain other permissions for your intended use. For example, other rights such as publicity, privacy or moral rights may limit how you may use the material."@en ;
  skos:note "Het is mogelijk dat je meer toestemming moet verkrijgen voor je beoogde gebruik. Bijvoorbeeld, andere rechten als publiciteitsrechten, privacy recht, of morele rechten kunnen het mogelijke gebruik van dit item beperken."@nl ;
  skos:note "You may find additional information about the copyright status of the item on the website of the organization that has made the item available."@en ;
  skos:note "Je kan aanvullende informatie over de rechtenstatus van het item op de website van de organisatie vinden die het item beschikbaar heeft gesteld."@nl ;
  skos:note "If you have any information that can contribute to identifying or locating the rights-holder(s) please notify the organization that has made the item available."@en ;
  skos:note "Neem contact op met de organisatie die dit item beschikbaar heeft gesteld als je enige informatie hebt over de auteursrechtelijk status van dit item dat kan bijdragen aan de identificering of localisering van de rechthebbende."@nl ;
  skos:scopeNote "This rights statement is intended for use with an item that has been identified as in copyright but for which no rights-holder(s) has been identified or located after some reasonable investigation. This rights statement should only be used if the data provider is reasonably sure that the work is in copyright. This rights statement is not intended for use by EU-based data providers who have identified works as Orphan Works in accordance with the EU Orphan Works Directive (they must use IC-OW-EU instead)."@en ;
  skos:relatedMatch premiscopy:cpr ;
  dcterms:creator <irswg> ;
  owl:versionInfo "0.0" ;
  dc:identifier "InC-RUU" ;
  skos:inScheme <0.0/> .

<InC-EDU/0.0/> a dcterms:RightsStatement, skos:Concept ;
  skos:prefLabel "In Copyright - Educational Use Permitted"@en ;
  skos:prefLabel "Beperkt door het Auteursrecht - Gebruik voor onderwijsdoeleinden toegestaan"@nl ;
  dcterms:isReplacedBy <InC-EDU/1.0/> ;
  dcterms:modified "2016-02-25"^^xsd:date ;
  skos:definition """This item is protected by copyright and/or related rights.

You are free to use this item in any way that is permitted by the copyright and related rights legislation that applies to your use. In addition, no permission is required from the rights-holder(s) for educational uses.

For other uses, you need to obtain permission from the rights-holder(s)."""@en ;
  skos:definition """Het gebruik van dit item wordt beperkt auteursrecht of aanverwante rechten.

Je bent vrij om dit item te gebruiken op de manier die toegestaan zijn door he auteursrecht en aanverwante rechten volgende de wetten die op jou van toepassing zijn. Additioneel is er voor educatief gebruik geen toestemming nodig van de rechthebbende.

Voor andere gebruiken heb je toestemming van de rechthebbende nodig."""@nl ;
  skos:note "Unless expressly stated otherwise, the organization that has made this item available makes no warranties about the item and cannot guarantee the accuracy of this rights statement. You are responsible for your own use."@en ;
  skos:note "Tenzij expliciet aangegeven, de organisatie die dit artikel beschikbaar heeft gesteld geeft geen garanties over het item. Je bent verantwoordelijk voor je eigen gebruik."@nl ;
  skos:note "You may need to obtain other permissions for your intended use. For example, other rights such as publicity, privacy or moral rights may limit how you may use the material."@en ;
  skos:note "Het is mogelijk dat je meer toestemming moet verkrijgen voor je beoogde gebruik. Bijvoorbeeld, andere rechten als publiciteitsrechten, privacy recht, of morele rechten kunnen het mogelijke gebruik van dit item beperken."@nl ;
  skos:note "You may find additional information about the copyright status of the item on the website of the organization that has made the item available."@en ;
  skos:note "Je kan aanvullende informatie over de rechtenstatus van het item op de website van de organisatie vinden die het item beschikbaar heeft gesteld."@nl ;
  skos:scopeNote "This rights statement can be used only for copyrighted items for which the organization making the item available is the rights-holder or has been explicitly authorized by the rights-holder(s) to allow third parties to use the work for educational purposes without first obtaining permission."@en ;
  skos:scopeNote "Deze rechtenstatement kan gebruikt worden voor elke auteursrechtelijke beschermd werk. De statemetn kan alleen toegepast worden wanneer de organisatie die deze statement aan het item verbind de rechthebbende is van het werk of expliciete toestemming heeft verkregen van de rechthebbende(n) om het werk beschikbaar te stellen voor educatief gebruik voor derden zonder daar zelf toestemming voor te hoeven vragen."@nl ;
  skos:relatedMatch premiscopy:cpr ;
  dcterms:creator <irswg> ;
  owl:versionInfo "0.0" ;
  dc:identifier "InC-EDU" ;
  skos:inScheme <0.0/> .

<InC-NC/0.0/> a dcterms:RightsStatement, skos:Concept ;
  skos:prefLabel "In Copyright - NonCommercial Use Permitted"@en ;
  skos:prefLabel "Gebruikt Beperkt door het Auteursrecht – Niet Commercieel Gebruik Toegestaan"@nl ;
  dcterms:isReplacedBy <InC-NC/1.0/> ;
  dcterms:modified "2016-02-25"^^xsd:date ;
  skos:definition """This item is protected by copyright and/or related rights. 

You are free to use this item in any way that is permitted by the copyright and related rights legislation that applies to your use. In addition, no permission is required from the rights-holder(s) for non-commercial uses.

For other uses you need to obtain permission from the rightsholder(s)."""@en ;
  skos:definition """Het gebruik van dit item wordt beperkt door het auteursrecht een aanverwante rechten.
  
Je bent vrij om dit item te gebruiken op manieren die worden toegestaan door de auteurswet of wetten op aanverwante rechten die op jou van toepassing zijn. Additioneel is er geen toestemming nodig van de rechthebbenden voor alle niet commerciele gebruiken.
  
Voor andere gebruiken heb je toestemming van de rechthebbende nodig."""@nl ;
  skos:note "Unless expressly stated otherwise, the organization that has made this item available makes no warranties about the item and cannot guarantee the accuracy of this rights statement. You are responsible for your own use."@en ;
  skos:note "Tenzij expliciet aangegeven, de organisatie die dit artikel beschikbaar heeft gesteld geeft geen garanties over het item. Je bent verantwoordelijk voor je eigen gebruik."@nl ;
  skos:note "You may need to obtain other permissions for your intended use. For example, other rights such as publicity, privacy or moral rights may limit how you may use the material."@en ;
  skos:note "Het is mogelijk dat je meer toestemming moet verkrijgen voor je beoogde gebruik. Bijvoorbeeld, andere rechten als publiciteitsrechten, privacy recht, of morele rechten kunnen het mogelijke gebruik van dit item beperken."@nl ;
  skos:note "You may find additional information about the copyright status of the item on the website of the organization that has made the item available."@en ;
  skos:note "Je kan aanvullende informatie over de rechtenstatus van het item op de website van de organisatie vinden die het item beschikbaar heeft gesteld."@nl ;
  skos:scopeNote "This rights statement can be used only for copyrighted items for which the organization making  the item available is the rights-holder or has been explicitly authorized by the rights-holder(s) to allow third parties to use the work for non-commercial purposes without obtaining permission first."@en ;
  skos:scopeNote "Deze rechtenstatement kan gebruikt worden voor elke auteursrechtelijke beschermd werk. De statemetn kan alleen toegepast worden wanneer de organisatie die deze statement aan het item verbind de rechthebbende is van het werk of expliciete toestemming heeft verkregen van de rechthebbende(n) om het werk beschikbaar te stellen voor niet commercieel gebruik door derden zonder dat deze toestemming hiervoor hoeven te vragen."@nl ;
  cc:prohibits cc:CommercialUse ;
  skos:closeMatch <http://creativecommons.org/licenses/by-nc/4.0/> ;
  skos:relatedMatch premiscopy:cpr ;
  dcterms:creator <irswg> ;
  owl:versionInfo "0.0" ;
  dc:identifier "InC-NC" ;
  skos:inScheme <0.0/> .

<NoC-CR> a dcterms:RightsStatement, skos:Concept ;
  skos:prefLabel "No Copyright - Contractual Restrictions"@en ;
  skos:prefLabel "Geen Auteursrechtelijke Beperkingen - Beperkt door Contractuele Beperkingen"@nl ;
  dcterms:isReplacedBy <NoC-CR/1.0/> ;
  dcterms:modified "2016-02-25"^^xsd:date ;
  skos:definition """Use of this item is not restricted by copyright and/or related rights.

As part of the acquisition or digitization of this item, the organization that has made the item available is contractually required to limit the use of this item. Limitations may include, but are not limited to, privacy issues, cultural protections, digitization agreements or donor agreements.

Please refer to the organization that has made the item available for more information."""@en ;
  skos:definition """Het gebruik van dit item is niet beperkt door het auteursrecht of naburige rechten.

De organisatie die dit item beschikbaar heeft gesteld moet door contractuele beperkingen het toegestane gebruik van het werk beperken als onderdeel van de acquisitie of digitalisering van dit item. Deze beperkingen kunnen ontstaan door privacy vraagstukken, culturele bescherming of door afspraken met donateurs.

Kijk bij de organisatie die dit item beschikbaar heeft gesteld voor meer informatie."""@nl ;
  skos:note "Unless expressly stated otherwise, the organization that has made this item available makes no warranties about the item and cannot guarantee the accuracy of this rights statement. You are responsible for your own use."@en ;
  skos:note "Tenzij expliciet aangegeven, de organisatie die dit artikel beschikbaar heeft gesteld geeft geen garanties over het item. Je bent verantwoordelijk voor je eigen gebruik."@nl ;
  skos:note "You may need to obtain other permissions for your intended use. For example, other rights such as publicity, privacy or moral rights may limit how you may use the material."@en ;
  skos:note "Het is mogelijk dat je meer toestemming moet verkrijgen voor je beoogde gebruik. Bijvoorbeeld, andere rechten als publiciteitsrechten, privacy recht, of morele rechten kunnen het mogelijke gebruik van dit item beperken."@nl ;
  skos:note "You may find additional information about the copyright status of the item on the website of the organization that has made the item available."@en ;
  skos:note "Je kan aanvullende informatie over de rechtenstatus van het item op de website van de organisatie vinden die het item beschikbaar heeft gesteld."@nl ;
  skos:scopeNote "This rights statement can only be used for items that are in the public domain but for which the data provider has entered into contractual agreement that requires it to take steps to restrict third party uses of the item. In order for this rights statement to be conclusive, the data provider must provide a link to a page detailing the the contractual restrictions that apply to the use of the item."@en ;
  skos:scopeNote "Deze rechtenstatement kan alleen gebruikt worden bij items die in het publiek domein zijn, maar waar de data provider een contractuele overeenkomst heeft gesloten die het gebruik door derde partijen beperkt. Om deze statement afdoende te maken moet de data provider een link toevoegen naar een webpagina die de contractuele beperking beschrijft."@nl ;
  skos:relatedMatch premiscopy:pub ;
  owl:versionInfo "0.0" ;
  dcterms:creator <irswg> ;
  dc:identifier "NoC-CR" ;
  skos:inScheme <0.0/> .

<NoC-OKLR/0.0/> a dcterms:RightsStatement, skos:Concept ;
  skos:prefLabel "No Copyright - Other Known Legal Restrictions"@en ;
  skos:prefLabel "Geen Auteursrechtelijke Beperking - Andere Juridische Beperkingen"@nl ;
  dcterms:isReplacedBy <NoC-OKLR/1.0/> ;
  dcterms:modified "2016-02-25"^^xsd:date ;
  skos:definition """Use of this item is not restricted by copyright and/or related rights.

In one or more jurisdictions, laws other than copyright are known to impose restrictions on the use of this item.

Please refer to the organization that has made the item available for more information."""@en ;
  skos:definition """Dit item heeft geen gebruiksbeperkingen gebaseerd op het auteursrecht of naburige rechten.

In één of meerdere jurisdicties kunnen er wetten bestaan buiten het auteursrecht die additionele gebruiksbeperkingen aan dit item.   

Kijk bij de organisatie die dit item beschikbaar heeft gesteld voor meer informatie."""@nl ;
  skos:note "Unless expressly stated otherwise, the organization that has made this item available makes no warranties about the item and cannot guarantee the accuracy of this rights statement. You are responsible for your own use."@en ;
  skos:note "Tenzij expliciet aangegeven, de organisatie die dit artikel beschikbaar heeft gesteld geeft geen garanties over het item. Je bent verantwoordelijk voor je eigen gebruik."@nl ;
  skos:note "You may need to obtain other permissions for your intended use. For example, other rights such as publicity, privacy or moral rights may limit how you may use the material."@en ;
  skos:note "Het is mogelijk dat je meer toestemming moet verkrijgen voor je beoogde gebruik. Bijvoorbeeld, andere rechten als publiciteitsrechten, privacy recht, of morele rechten kunnen het mogelijke gebruik van dit item beperken."@nl ;
  skos:note "You may find additional information about the copyright status of the item on the website of the organization that has made the item available."@en ;
  skos:note "Je kan aanvullende informatie over de rechtenstatus van het item op de website van de organisatie vinden die het item beschikbaar heeft gesteld."@nl ;
  skos:scopeNote "This rights statement should be used for items that are in the public domain but that cannot be freely re-used as the consequence of known legal restrictions that prevent the data provider from allowing free re-use of the work, such as cultural heritage or traditional cultural expression protections. In order for this rights statement to be conclusive, the data provider must provide a link to a page detailing the the legal restrictions that limit re-use of the item."@en ;
  skos:scopeNote "Deze rechtenstatement kan alleen gebruikt worden bij items die in het publiek domein zijn, maar als een consequentie van andere juridische restricties niet gedeeld kan worden voor hergebruik door de data provider. Om deze statement afdoende te maken moet de data provider een link toevoegen naar een webpagina die de contractuele beperking beschrijft."@nl ;
  skos:relatedMatch premiscopy:pub ;
  owl:versionInfo "0.0" ;
  dcterms:creator <irswg> ;
  dc:identifier "NoC-OKLR" ;
  skos:inScheme <0.0/> .

<NKC/0.0/> a dcterms:RightsStatement, skos:Concept ;
  skos:prefLabel "No Known Copyright"@en ;
  skos:prefLabel "Geen Bekende Auteursrechtelijke Beperking"@nl ;
  dcterms:isReplacedBy <NKC/1.0/> ;
  dcterms:modified "2016-02-25"^^xsd:date ;
  skos:definition """The organization that has made the item available reasonably believes that the item is not restricted by copyright or related rights, but a conclusive determination could not be made. 

Please refer to the organization that has made the item available for more information. 

You are free to use this item in any way that is permitted by the copyright and related rights legislation that applies to your use."""@en ;
  skos:note "Unless expressly stated otherwise, the organization that has made this item available makes no warranties about the item and cannot guarantee the accuracy of this rights statement. You are responsible for your own use."@en ;
  skos:definition """De organisatie die dit item beschikbaar heeft gesteld heeft reden om te geloven dat er geen auteursrechtelijke beperkingen of beperkingen door naburige rechten bestaan voor dit item, maar een definitie determinatie kon niet worden gemaakt. Kijk bij de organisatie die dit item beschikbaar heeft gesteld voor meer informatie. 

Je bent vrij om dit item te gebruiken op manieren die worden toegestaan door de auteurswet of wetten op aanverwante rechten die op jou van toepassing zijn."""@nl ;
  skos:note "Tenzij expliciet aangegeven, de organisatie die dit artikel beschikbaar heeft gesteld geeft geen garanties over het item. Je bent verantwoordelijk voor je eigen gebruik."@nl ;
  skos:note "You may need to obtain other permissions for your intended use. For example, other rights such as publicity, privacy or moral rights may limit how you may use the material."@en ;
  skos:note "Het is mogelijk dat je meer toestemming moet verkrijgen voor je beoogde gebruik. Bijvoorbeeld, andere rechten als publiciteitsrechten, privacy recht, of morele rechten kunnen het mogelijke gebruik van dit item beperken."@nl ;
  skos:note "You may find additional information about the copyright status of the item on the website of the organization that has made the item available."@en ;
  skos:note "Je kan aanvullende informatie over de rechtenstatus van het item op de website van de organisatie vinden die het item beschikbaar heeft gesteld."@nl ;
  skos:scopeNote "This rights statement should be used for items for which the copyright status has not been determined conclusively, but for which the data provider has reasonable cause to believe that the work is not covered by copyright or related rights anymore. This rights statement should not be used for orphan works (which are assumed to be in-copyright) or for works where the data provider has not undertaken an effort to ascertain the copyright status of the work."@en ;
  skos:scopeNote "Dit rechtenstatement kan alleen gebruikt worden bij items waar de auteursrechtelijke status niet definitief te bepalen is, maar waar de data provider redelijkerwijs kan stellen dat de het item niet langer door auteursrechten of naburige rechten beperkt wordt, Dit rechtenstatement moet niet gebruikt worden bij verweesde werken (waar aangenomen kan worden dat deze nog auteursrechtelijk beperkt zijn) en voor werken waar de data provider geen poging ondernomen heeft om de auteursrechtelijke status van het werk vast te stellen"@nl ;
  skos:relatedMatch premiscopy:unk ;
  owl:versionInfo "0.0" ;
  dcterms:creator <irswg> ;
  dc:identifier "NKC" ;
  skos:inScheme <0.0/> .

<CNE/0.0/> a dcterms:RightsStatement, skos:Concept ;
  skos:prefLabel "Copyright Not Evaluated"@en ;
  skos:prefLabel "Auteursrechtelijke Status niet beoordeeld."@nl ;
  dcterms:isReplacedBy <CNE/1.0/> ;
  dcterms:modified "2016-02-25"^^xsd:date ;
  skos:definition """The copyright and related rights status of this item has not been evaluated. 

Please refer to the organization that has made the item available for more information. 

You are free to use this item in any way that is permitted by the copyright and related rights legislation that applies to your use."""@en ;
  skos:definition """De auteursrechtelijke status en de naburige rechten status van dit item zijn niet geïdentificeerd. Kijk bij de organisatie die dit item beschikbaar heeft gesteld voor meer informatie.
  
Je bent vrij om dit item te gebruiken op manieren die worden toegestaan door de auteurswet of wetten op aanverwante rechten die op jou van toepassing zijn."""@nl ;
  skos:note "Unless expressly stated otherwise, the organization that has made this item available makes no warranties about the item and cannot guarantee the accuracy of this rights statement. You are responsible for your own use."@en ;
  skos:note "Tenzij expliciet aangegeven, de organisatie die dit artikel beschikbaar heeft gesteld geeft geen garanties over het item. Je bent verantwoordelijk voor je eigen gebruik."@nl ;
  skos:note "You may need to obtain other permissions for your intended use. For example, other rights such as publicity, privacy or moral rights may limit how you may use the material."@en ;
  skos:note "Het is mogelijk dat je meer toestemming moet verkrijgen voor je beoogde gebruik. Bijvoorbeeld, andere rechten als publiciteitsrechten, privacy recht, of morele rechten kunnen het mogelijke gebruik van dit item beperken."@nl ;
  skos:note "You may find additional information about the copyright status of the item on the website of the organization that has made the item available."@en ;
  skos:note "Je kan aanvullende informatie over de rechtenstatus van het item op de website van de organisatie vinden die het item beschikbaar heeft gesteld."@nl ;
  skos:scopeNote "This rights statement should be used for items for which the copyright status is unknown and for which the data provider has not undertaken an effort to determine the copyright status of the work."@en ;
  skos:scopeNote "Dit rechtenstatement kan alleen gebruikt worden bij items waar de auteursrechtelijke status onbekend is en waar de data provider geen poging ondernomen heeft om de auteursrechtelijke status van het werk te bepalen."@nl ;
  skos:closeMatch <http://www.europeana.eu/rights/unknown/> ;
  skos:relatedMatch premiscopy:unk ;
  owl:versionInfo "0.0" ;
  dcterms:creator <irswg> ;
  dc:identifier "CNE" ;
  skos:inScheme <0.0/> .
